ballet/63/examples/function_test/application.e
@@ -1,0 +1,46 @@
+indexing
+	description : "function_test application root class"
+	date        : "$Date$"
+	revision    : "$Revision$"
+
+class
+	APPLICATION
+
+inherit
+	ARGUMENTS
+
+create
+	make
+
+feature {NONE} -- Initialization
+
+	make
+			-- Run application.
+		local
+			l_agent: FUNCTION [ANY, TUPLE [INTEGER, INTEGER], INTEGER]
+			l_result: INTEGER
+		do
+			l_agent := agent addition
+			l_result := apply_function (l_agent)
+			check l_result = 3 end
+		end
+
+
+
+	addition (a, b: INTEGER): INTEGER
+		do
+			Result := a + b
+		ensure
+			Result = a + b
+		end
+
+	apply_function (f: FUNCTION [ANY, TUPLE [INTEGER, INTEGER], INTEGER]): INTEGER
+		require
+			f.precondition ([1, 2])
+		do
+			Result := f.item ([1, 2])
+		ensure
+			f.postcondition ([1, 2])
+		end
+
+end
